Modify the definition of the set of type variables

Types.v
@@ -17,18 +17,18 @@ Qed.
 Definition typ_eqMixin := EqMixin typ_eqP.
 Canonical typ_eqType := Eval hnf in EqType typ typ_eqMixin.
 
-Fixpoint typ_fv T :=
+Fixpoint typ_fv T : pred nat :=
   match T with
-  | typ_fvar x => [:: x]
-  | typ_bvar _ => [::]
-  | typ_arrow T1 T2 => typ_fv T1 ++ typ_fv T2
+  | typ_fvar x => pred1 x
+  | typ_bvar _ => pred0
+  | typ_arrow T1 T2 => predU (typ_fv T1) (typ_fv T2)
   end.
 
-Fixpoint typ_bv T :=
+Fixpoint typ_bv T : pred nat :=
   match T with
-  | typ_fvar _ => [::]
-  | typ_bvar x => [:: x]
-  | typ_arrow T1 T2 => typ_bv T1 ++ typ_bv T2
+  | typ_fvar _ => pred0
+  | typ_bvar x => pred1 x
+  | typ_arrow T1 T2 => predU (typ_bv T1) (typ_bv T2)
   end.
 
 Fixpoint typ_subst s T :=
@@ -63,9 +63,10 @@ Lemma typ_subst_ext s s' T :
   typ_subst s T = typ_subst s' T.
 Proof.
   induction T => //= [ | Hext ].
-  - apply. by rewrite mem_seq1 eq_refl.
-  - f_equal; [ apply /IHT1 | apply /IHT2 ] => ? Hfv;
-    apply /Hext; by rewrite mem_cat Hfv ?orbT.
+  - apply. by rewrite inE eqxx.
+  - f_equal; [ apply /IHT1 | apply /IHT2 ] => ?;
+    rewrite -topredE => /= Hfv; apply /Hext;
+    by rewrite inE Hfv ?orbT.
 Qed.
 
 Corollary typ_subst_fvar_eq s T :
@@ -86,9 +87,9 @@ Lemma typ_fv_subst s T x :
 Proof.
   induction T => //= [ Hin | ].
   - exists x0.
-    by rewrite Hin mem_seq1 eq_refl.
-  - rewrite mem_cat => /orP [ /IHT1 | /IHT2 ] [ y [ Hs Hfv ] ];
-    exists y; by rewrite Hs mem_cat Hfv ?orbT.
+    by rewrite Hin inE eqxx.
+  - rewrite inE => /orP [ /IHT1 | /IHT2 ] [ y [ Hs ] ];
+    rewrite -topredE => /= Hfv; exists y; by rewrite Hs inE Hfv ?orbT.
 Qed.
 
 Lemma typ_fv_subst_intro s T x y :
@@ -97,9 +98,9 @@ Lemma typ_fv_subst_intro s T x y :
   x \in typ_fv (typ_subst s T).
 Proof.
   induction T => //=.
-  - by rewrite mem_seq1 => /eqP ->.
-  - rewrite !mem_cat => /orP [ ] Hin => [ /(IHT1 Hin) | /(IHT2 Hin) ] -> //.
-    by rewrite orbT.
+  - by rewrite inE => /eqP ->.
+  - rewrite inE => /orP [ ] Hin => [ /(IHT1 Hin) | /(IHT2 Hin) ];
+    rewrite inE -topredE => /= -> //; by rewrite orbT.
 Qed.
 
 Lemma typ_bv_subst s T x :
@@ -107,9 +108,10 @@ Lemma typ_bv_subst s T x :
   x \in typ_bv T \/ exists y, x \in typ_bv (s y) /\ y \in typ_fv T.
 Proof.
   induction T => /= [ Hin | | ]; eauto.
-  - right. exists x0. rewrite mem_seq1 eqxx. eauto.
-  - rewrite !mem_cat => /orP [ /IHT1 | /IHT2 ] [ -> | [ y [ Hs Hfv ] ] ]; rewrite ?orbT; eauto;
-    right; exists y; by rewrite Hs mem_cat Hfv ?orbT.
+  - right. exists x0. rewrite inE eqxx. eauto.
+  - rewrite !inE => /orP [ /IHT1 | /IHT2 ];
+    (move => [ | [ y [ Hs ] ] ]; rewrite -topredE) => /= [ -> | Hfv ]; rewrite ?orbT; eauto;
+    right; exists y; by rewrite Hs inE Hfv ?orbT.
 Qed.
 
 Lemma typ_bv_subst_intro_sub s T x y :
@@ -118,9 +120,9 @@ Lemma typ_bv_subst_intro_sub s T x y :
   x \in typ_bv (typ_subst s T).
 Proof.
   induction T => //=.
-  - by rewrite mem_seq1 => /eqP ->.
-  - rewrite !mem_cat => /orP [ ] Hin => [ /(IHT1 Hin) | /(IHT2 Hin) ] -> //.
-    by rewrite orbT.
+  - by rewrite inE => /eqP ->.
+  - rewrite !inE => /orP [ ] Hin => [ /(IHT1 Hin) | /(IHT2 Hin) ];
+    rewrite -topredE => /= -> //; by rewrite orbT.
 Qed.
 
 Lemma typ_open_bvar T : typ_open typ_bvar T = T.
@@ -131,9 +133,9 @@ Lemma typ_open_ext s s' T :
   typ_open s T = typ_open s' T.
 Proof.
   induction T => //= [ | Hext ].
-  - apply. by rewrite mem_seq1 eqxx.
-  - congr (typ_arrow _ _); [ apply /IHT1 | apply /IHT2 ] => ? Hin;
-    apply /Hext; by rewrite mem_cat Hin ?orbT.
+  - apply. by rewrite inE eqxx.
+  - congr (typ_arrow _ _); [ apply /IHT1 | apply /IHT2 ] => ?;
+    rewrite -topredE => /= Hin; apply /Hext; by rewrite inE Hin ?orbT.
 Qed.
 
 Corollary typ_open_bvar_eq s T :
@@ -153,19 +155,20 @@ Lemma typ_bv_open s T x :
 Proof.
   induction T => //= [ Hin | ].
   - exists n.
-    by rewrite Hin mem_seq1 eqxx.
-  - rewrite mem_cat => /orP [ /IHT1 | /IHT2 ] [ y [ Hs Hfv ] ];
-    exists y; by rewrite Hs mem_cat Hfv ?orbT.
+    by rewrite Hin inE eqxx.
+  - rewrite inE => /orP [ /IHT1 | /IHT2 ] [ y [ Hs ] ];
+    rewrite -topredE => /= Hbv; exists y; by rewrite Hs inE Hbv ?orbT.
 Qed.
 
 Lemma typ_fv_open s T x :
   x \in typ_fv (typ_open s T) ->
   x \in typ_fv T \/ exists y, x \in typ_fv (s y) /\ y \in typ_bv T.
 Proof.
-  induction T => /= [ Hin | | ]; eauto.
-  - right. exists n. rewrite mem_seq1 eqxx. eauto.
-  - rewrite !mem_cat => /orP [ /IHT1 | /IHT2 ] [ -> | [ y [ Hs Hfv ] ] ]; rewrite ?orbT; eauto;
-    right; exists y; by rewrite Hs mem_cat Hfv ?orbT.
+  induction T => /= [ ? | | ]; eauto.
+  - right. exists n. rewrite inE eqxx. eauto.
+  - rewrite !inE => /orP [ /IHT1 | /IHT2 ];
+    (move => [ | [ y [ Hs ] ] ]; rewrite -topredE) => /= [ -> | Hbv ]; rewrite ?orbT; eauto;
+    right; exists y; by rewrite Hs inE Hbv ?orbT.
 Qed.
 
 Lemma typ_subst_open_distr s s' T :
@@ -174,9 +177,10 @@ Lemma typ_subst_open_distr s s' T :
 Proof.
   induction T => //= Hclose.
   - rewrite typ_open_bvar_eq => //= ? ?.
-    by rewrite (Hclose x) // mem_seq1 eqxx.
-  - congr (typ_arrow _ _ ); [ rewrite IHT1 | rewrite IHT2 ] => // ? Hin ?;
-    apply /Hclose; by rewrite mem_cat Hin ?orbT.
+    by rewrite (Hclose x) // inE eqxx.
+  - congr (typ_arrow _ _ ); [ rewrite IHT1 | rewrite IHT2 ] => // ?;
+    rewrite -topredE => /= Hin ?;
+    apply /Hclose; by rewrite inE Hin ?orbT.
 Qed.
 
 Lemma typ_open_subst_distr s s' T :
@@ -185,9 +189,10 @@ Lemma typ_open_subst_distr s s' T :
 Proof.
   induction T => //= Hfresh.
   - rewrite typ_subst_fvar_eq => //= ? ?.
-    by rewrite (Hfresh n) //= mem_seq1 eqxx.
-  - congr (typ_arrow _ _ ); [ rewrite IHT1 | rewrite IHT2 ] => // ? Hin ?;
-    apply /Hfresh; by rewrite mem_cat Hin ?orbT.
+    by rewrite (Hfresh n) //= inE eqxx.
+  - congr (typ_arrow _ _ ); [ rewrite IHT1 | rewrite IHT2 ] => // ?;
+    rewrite -topredE => /= Hin ?;
+    apply /Hfresh; by rewrite inE Hin ?orbT.
 Qed.
 
 
@@ -202,9 +207,9 @@ Lemma unifies_occur_aux s x : forall T,
   x \in typ_fv T -> typ_size (typ_subst s T) <= typ_size (s x) -> T = typ_fvar x.
 Proof.
   elim => /= [ ? | ? | ? IHT1 ? IHT2 ].
-  - by rewrite mem_seq1 => /eqP <-.
-  - by rewrite in_nil.
-  - rewrite mem_cat => /orP [ /IHT1 | /IHT2 ] IH Hsize;
+  - by rewrite inE => /eqP <-.
+  - by rewrite inE.
+  - rewrite inE => /orP [ /IHT1 | /IHT2 ] IH Hsize;
     move: IH (Hsize) => -> /=.
     + by rewrite ltnNge leq_addr.
     + exact: (leq_trans (leq_addr _ _) (ltnW Hsize)).
@@ -245,20 +250,6 @@ Proof.
     by rewrite -IH.
 Qed.
 
-Fixpoint typ_occur x T :=
-  match T with
-  | typ_fvar y => x == y
-  | typ_bvar _ => false
-  | typ_arrow T1 T2 => (typ_occur x T1) || (typ_occur x T2)
-  end.
-
-Lemma typ_occur_fv x : forall T, typ_occur x T = (x \in typ_fv T).
-Proof.
-  elim => //= [ ? | ? -> ? -> ].
-  - by rewrite mem_seq1.
-  - by rewrite mem_cat.
-Qed.
-
 Section UnifyInner.
   Variable unify : typ -> typ -> seq (nat * typ) -> option (seq (nat * typ)).
 
@@ -277,7 +268,7 @@ Section UnifyInner.
   Definition flex_rigid x T2 s :=
     match s with
     | [::] =>
-        if typ_occur x T2 then None
+        if x \in typ_fv T2 then None
         else Some [:: (x, T2)]
     | (z, T) :: s =>
         omap (cons (z, T))
@@ -311,8 +302,7 @@ Section UnifyInner.
     typ_subst_seq (typ_fvar x) s' = typ_subst_seq T2 s'.
   Proof.
     move => [ | [ z T ] s ] /=.
-    - rewrite typ_occur_fv.
-      destruct (x \in typ_fv T2) eqn:Hin; inversion 1 => /=.
+    - destruct (x \in typ_fv T2) eqn:Hin; inversion 1 => /=.
       rewrite eqxx typ_subst_single_notin ?Hin; eauto.
     - destruct
         (unify (if x == z then T else typ_fvar x)
@@ -327,7 +317,7 @@ Section UnifyInner.
     typ_subst_seq (typ_fvar x) s' = typ_subst_seq (typ_fvar y) s'.
   Proof.
     move: (flex_rigid_sound x (typ_fvar y) s' s).
-    rewrite /flex_flex /flex_rigid /=.
+    rewrite /flex_flex /flex_rigid /= inE.
     case (@eqP _ x y); eauto.
     inversion 3. subst.
     exists [::]. by rewrite cats0.
@@ -389,9 +379,8 @@ Section UnifyInner.
   Proof.
     move => [ | [ z T ] s ] /= s' Huniq =>
       [ ? | [ /andP [ Hz Hoccur ] [ HT Hvalid ] ] ] Hx HT2 Hunifies => [ | ? ].
-    - rewrite typ_occur_fv.
-      destruct (x \in typ_fv T2) eqn:Hoccur.
-      { by rewrite (unifies_occur _ _ _ Hunifies Hoccur) eq_refl. }
+    - destruct (x \in typ_fv T2) eqn:Hoccur.
+      { by rewrite (unifies_occur _ _ _ Hunifies Hoccur) eqxx. }
       exists [:: (x, T2)] => /=. rewrite Hx Hoccur. repeat split; eauto.
       exists s' => ?.
       rewrite typ_subst_comp.
@@ -407,13 +396,13 @@ Section UnifyInner.
         case (@eqP _ x z) => [ | /eqP ] ? /=; subst.
         - case (@eqP _ y z) => [ -> | ? /HT // ].
           by rewrite (negbTE Hoccur).
-        - rewrite mem_seq1 => /eqP ?. subst.
+        - rewrite inE => /eqP ?. subst.
           by rewrite Hx andbT. }
       { rewrite rem_filter // mem_filter /= => /typ_fv_subst /= [ w [ ] ].
         case (@eqP _ w z) => /= [ | /eqP ] ?; subst.
         - case (@eqP _ y z) => /= [ -> | ? /HT // ].
           by rewrite (negbTE Hoccur).
-        - rewrite mem_seq1 => /eqP -> /HT2 ->.
+        - rewrite inE => /eqP -> /HT2 ->.
           by rewrite andbT. }
       eauto 6.
   Qed.
@@ -433,11 +422,11 @@ Section UnifyInner.
   Proof.
     move => ? ? ? Hy ?.
     move: (flex_rigid_complete x (typ_fvar y) s s').
-    rewrite /flex_rigid /flex_flex /=.
+    rewrite /flex_rigid /flex_flex /= inE.
     case (@eqP _ x y) => ?; subst.
     - exists [::]. rewrite cats0. eauto.
     - apply => // [ ? | ].
-      + rewrite mem_seq1 => /eqP ?. by subst.
+      + rewrite inE => /eqP ?. by subst.
       + apply /eqP. congruence.
   Qed.
 
@@ -456,28 +445,28 @@ Section UnifyInner.
   Proof.
     elim => [ x | x | T11 IHT11 T12 IHT12 ] [ y | y | T21 T22 ] /= s s' Huniq Hvalid HT1 HT2 Hunifies.
     - apply /flex_flex_complete => //=.
-      + apply /HT1. by rewrite mem_seq1.
-      + apply /HT2. by rewrite mem_seq1.
+      + apply /HT1. by rewrite inE.
+      + apply /HT2. by rewrite inE.
     - apply /flex_rigid_complete => //=.
-      apply /HT1. by rewrite mem_seq1.
+      apply /HT1. by rewrite inE.
     - apply /flex_rigid_complete => //=.
-      apply /HT1. by rewrite mem_seq1.
+      apply /HT1. by rewrite inE.
     - apply /flex_rigid_complete => //=.
-      apply /HT2. by rewrite mem_seq1.
+      apply /HT2. by rewrite inE.
     - case (@eqP _ x y).
       + exists [::]. rewrite cats0. eauto.
       + move: Hunifies. rewrite !typ_subst_seq_bvar /=. congruence.
     - move: Hunifies. rewrite typ_subst_seq_arrow typ_subst_seq_bvar //.
     - apply /flex_rigid_complete => //=.
-      apply /HT2. by rewrite mem_seq1.
+      apply /HT2. by rewrite inE.
     - move: Hunifies. rewrite typ_subst_seq_arrow typ_subst_seq_bvar //.
     - move: Hunifies. rewrite !typ_subst_seq_arrow. inversion 1.
-      case (IHT12 T22 s s') => // [ ? Hin | ? Hin | sd [ ? [ -> /= [ s'' Hgen ] ] ] ].
-      { by rewrite HT1 // mem_cat Hin orbT. }
-      { by rewrite HT2 // mem_cat Hin orbT. }
-      case (IHT11 T21 (s ++ sd) s'') => // [ ? Hin | ? Hin | | ? [ ] ].
-      { by rewrite HT1 // mem_cat Hin. }
-      { by rewrite HT2 // mem_cat Hin. }
+      case (IHT12 T22 s s') => // [ ? | ? | sd [ ? [ -> /= [ s'' Hgen ] ] ] ].
+      { rewrite -topredE => /= Hin. by rewrite HT1 // inE Hin orbT. }
+      { rewrite -topredE => /= Hin. by rewrite HT2 // inE Hin orbT. }
+      case (IHT11 T21 (s ++ sd) s'') => // [ ? | ? | | ? [ ] ].
+      { rewrite -topredE => /= Hin. by rewrite HT1 // inE Hin. }
+      { rewrite -topredE => /= Hin. by rewrite HT2 // inE Hin. }
       { by rewrite !typ_subst_seq_cat -!Hgen. }
       rewrite -!catA => ? [ -> [ sd' Hgen' ] ].
       (repeat eexists; eauto) => ?.
@@ -502,7 +491,7 @@ Section UnifyInner.
     bound_subst_seq s'.
   Proof.
     move => [ ? ? /= | [ z T ] s /= [ HT ? ] HT2 ].
-    - by case (typ_occur x T2); inversion 1.
+    - by case (x \in typ_fv T2); inversion 1.
     - destruct (unify (if x == z then T else typ_fvar x) (typ_subst [eta typ_fvar with z |-> T] T2)) eqn:Hunify; inversion 1.
       split; eauto.
       refine (typ_bv_unify _ _ _ _ _ _ _ Hunify) => // ? => [ | /typ_bv_subst [ /HT2 // | [ y [ /= ] ] ] ].
@@ -516,7 +505,7 @@ Section UnifyInner.
     bound_subst_seq s'.
   Proof.
     move: (flex_rigid_bound x (typ_fvar y) s' s).
-    rewrite /flex_rigid /flex_flex /=.
+    rewrite /flex_rigid /flex_flex /= inE.
     case (x == y) => [ | Hflex_rigid ? ].
     - inversion 3. subst. eauto.
     - exact /Hflex_rigid.
@@ -535,11 +524,12 @@ Section UnifyInner.
       | T11 IHT11 T12 IHT12 [ ? ? ? ? ? ? /flex_rigid_bound | | T21 T22 s ? ? HT1 HT2 ] ] //=; eauto.
     - by case (x == y); inversion 1; subst.
     - destruct (typ_unify_inner T12 T22 s) eqn:Hunify => //=.
-      apply /IHT11 => [ | ? Hin | ? Hin ].
-      + refine (IHT12 _ _ _ _ _ _ Hunify) => // ? Hin;
-        [ apply /HT1 | apply /HT2 ]; by rewrite /= mem_cat Hin orbT.
-      + apply /HT1. by rewrite /= mem_cat Hin.
-      + apply /HT2. by rewrite /= mem_cat Hin.
+      apply /IHT11 => [ | ? | ? ].
+      + refine (IHT12 _ _ _ _ _ _ Hunify) => // ?;
+        rewrite -topredE => /= Hin;
+        [ apply /HT1 | apply /HT2 ]; by rewrite /= inE Hin orbT.
+      + rewrite -topredE => /= Hin. apply /HT1. by rewrite /= inE Hin.
+      + rewrite -topredE => /= Hin. apply /HT2. by rewrite /= inE Hin.
   Qed.
 End UnifyInner.
 
@@ -599,8 +589,36 @@ Proof.
   - exact /typ_unify_inner_bound.
 Qed.
 
+Fixpoint typ_enum_fv acc T :=
+  match T with
+  | typ_fvar x => x :: acc
+  | typ_bvar x => acc
+  | typ_arrow T1 T2 => typ_enum_fv (typ_enum_fv acc T2) T1
+  end.
+
+Fixpoint typ_enum_bv acc T :=
+  match T with
+  | typ_fvar x => acc
+  | typ_bvar x => x :: acc
+  | typ_arrow T1 T2 => typ_enum_bv (typ_enum_bv acc T2) T1
+  end.
+
+Lemma typ_enum_fv_inE x : forall T acc,
+  (x \in typ_enum_fv acc T) = (x \in typ_fv T) || (x \in acc).
+Proof.
+  elim => //= ? IHT1 ? IHT2 ?.
+  by rewrite IHT1 IHT2 inE orbA.
+Qed.
+
+Lemma typ_enum_bv_inE x : forall T acc,
+  (x \in typ_enum_bv acc T) = (x \in typ_bv T) || (x \in acc).
+Proof.
+  elim => //= ? IHT1 ? IHT2 ?.
+  by rewrite IHT1 IHT2 inE orbA.
+Qed.
+
 Definition typ_unify T1 T2 :=
-  omap (fun s => typ_subst_seq^~s \o typ_fvar) (typ_unify_outer (size (typ_fv T1) + size (typ_fv T2)) T1 T2 [::]).
+  omap (fun s => typ_subst_seq^~s \o typ_fvar) (typ_unify_outer (size (typ_enum_fv (typ_enum_fv [::] T2) T1)) T1 T2 [::]).
 
 Lemma valid_subst_seq_fv : forall s L,
   uniq L ->
@@ -610,7 +628,7 @@ Proof.
   elim => /= [ ? ? ? ? ? -> // | [ y ? ] ? IH ? Huniq [ /andP [ ? ? ] [ HT0 Hvalid ] ] ? ? /(IH _ (rem_uniq _ Huniq) Hvalid) /orP [ /typ_fv_subst /= [ x [ ] ] | ] ].
   - case (@eqP _ x y) => /= [ -> /HT0 -> | ? ].
     + by rewrite orbT.
-    + by rewrite mem_seq1 => /eqP -> ->.
+    + by rewrite inE => /eqP -> ->.
   - rewrite (rem_filter _ Huniq) mem_filter => /= /andP [ ? -> ].
     by rewrite orbT.
 Qed.
@@ -620,7 +638,7 @@ Theorem typ_unify_sound T1 T2 s :
   typ_subst s T1 = typ_subst s T2.
 Proof.
   rewrite /typ_unify.
-  destruct (typ_unify_outer (size (typ_fv T1) + size (typ_fv T2)) T1 T2 [::]) eqn:Hunify; inversion 1. subst.
+  destruct (typ_unify_outer (size (typ_enum_fv (typ_enum_fv [::] T2) T1)) T1 T2 [::]) eqn:Hunify; inversion 1. subst.
   move: (typ_unify_outer_sound _ _ _ _ _ Hunify) => /= [ ? [ ?  ] ].
   by rewrite !typ_subst_seq_typ_subst.
 Qed.
@@ -633,16 +651,16 @@ Lemma typ_unify_complete_aux T1 T2 s :
 Proof.
   move => Hunifies.
   rewrite /typ_unify.
-  case (typ_unify_outer_complete (undup (typ_fv T1 ++ typ_fv T2)) (size (typ_fv T1) + size (typ_fv T2)) [::] s T1 T2)
+  case (typ_unify_outer_complete (undup (typ_enum_fv (typ_enum_fv [::] T2) T1)) (size (typ_enum_fv (typ_enum_fv [::] T2) T1)) [::] s T1 T2)
     => //= [ | | ? | ? | ? [ Hvalid [ -> [ ? Hgen ] ] ] ].
-  - by rewrite -size_cat size_undup.
+  - by rewrite size_undup.
   - exact: undup_uniq.
-  - by rewrite mem_undup mem_cat => ->.
-  - rewrite mem_undup mem_cat => ->. exact: orbT.
+  - by rewrite mem_undup typ_enum_fv_inE => ->.
+  - rewrite mem_undup !typ_enum_fv_inE => ->. exact: orbT.
   - (repeat eexists) => [ ? | ? ? /(valid_subst_seq_fv _ _ (undup_uniq _) Hvalid) /= /orP [ ] ].
     + by rewrite Hgen typ_subst_seq_typ_subst.
-    + rewrite mem_seq1 => /eqP; eauto.
-    + rewrite mem_undup mem_cat => /orP [ -> | -> ]; eauto.
+    + rewrite inE => /eqP; eauto.
+    + rewrite mem_undup !typ_enum_fv_inE in_nil => /orP [ -> | /orP [ -> | // ] ]; eauto.
 Qed.
 
 Theorem typ_unify_complete T1 T2 s :
@@ -671,9 +689,10 @@ Proof.
     - apply.
     - apply /IH => // ? /typ_bv_subst [ /HT | [ x [ ] ] ] //=.
       by case (x == y) => // /HT0. }
-  destruct (typ_unify_outer (size (typ_fv T1) + size (typ_fv T2)) T1 T2 [::]) eqn:Hunify; inversion 1 => ? x Hbv.
-  apply /orP. rewrite -mem_cat.
-  apply: H Hbv => //.
-apply: typ_unify_outer_bound Hunify => // ?; rewrite mem_cat => -> //.
-  by rewrite orbT.
+  destruct (typ_unify_outer (size (typ_enum_fv (typ_enum_fv [::] T2) T1)) T1 T2 [::]) eqn:Hunify; inversion 1 => ? x Hbv.
+  have : x \in typ_enum_bv (typ_enum_bv [::] T2) T1.
+  { apply: H Hbv => //.
+    apply: typ_unify_outer_bound Hunify => // ?; rewrite !typ_enum_bv_inE => -> //.
+    by rewrite orbT. }
+  rewrite !typ_enum_bv_inE in_nil => /orP [ -> | /orP [ -> | // ] ]; eauto.
 Qed.
